Substitution 1

lean/language.lean
@@ -31,7 +31,7 @@ begin
   finish,
 end
 
-@[simp] lemma update_apply_ne (name name' : string) (val : ℕ) (s : state)
+@[simp] lemma state.update_apply_ne (name name' : string) (val : ℕ) (s : state)
     (h : name' ≠ name) :
   s{name ↦ val} name' = s name' :=
 begin
@@ -39,7 +39,7 @@ begin
   exact if_neg h,
 end
 
-@[simp] lemma update_override (name : string) (val₁ val₂ : ℕ) (s : state) :
+@[simp] lemma state.update_override (name : string) (val₁ val₂ : ℕ) (s : state) :
   s{name ↦ val₂}{name ↦ val₁} = s{name ↦ val₁} :=
 begin
   apply funext,
@@ -48,7 +48,7 @@ begin
     simp [h]
 end
 
-@[simp] lemma update_swap (name₁ name₂ : string) (val₁ val₂ : ℕ) (s : state)
+@[simp] lemma state.update_swap (name₁ name₂ : string) (val₁ val₂ : ℕ) (s : state)
     (h : name₁ ≠ name₂ . tactic.dec_trivial) :
   s{name₂ ↦ val₂}{name₁ ↦ val₁} = s{name₁ ↦ val₁}{name₂ ↦ val₂} :=
 begin
@@ -59,7 +59,7 @@ begin
     simp * at *
 end
 
-@[simp] lemma update_id (name : string) (s : state) :
+@[simp] lemma state.update_id (name : string) (s : state) :
   s{name ↦ s name} = s :=
 begin
   apply funext,
@@ -68,7 +68,7 @@ begin
     simp * at *
 end
 
-@[simp] lemma update_same_const (name : string) (val : ℕ) :
+@[simp] lemma state.update_same_const (name : string) (val : ℕ) :
   (λ_, val){name ↦ val} = (λ_, val) :=
 by apply funext; simp
 
@@ -89,7 +89,7 @@ inductive stmt : Type
 | seq             : stmt → stmt → stmt
 | choice          : stmt → stmt → stmt
 | star            : stmt → stmt
-| local_var       : string → stmt → stmt
+-- | local_var       : string → stmt → stmt
 | error           : stmt
 | assumes         : prop → stmt
 
@@ -145,8 +145,8 @@ inductive lang_semantics: IncLoLang.stmt -> LogicType -> IncLoLang.state -> IncL
   lang_semantics (C₁ <+> C₂) ty s₁ s₂
 | star {C s₁ s₂ ty} (i: ℕ) (h: lang_semantics (repeat C i) ty s₁ s₂):
   lang_semantics (C**) ty s₁ s₂
-| local_var {C s₁ s₂ ty} (x: string) (v: ℕ) (h: lang_semantics C ty s₁ s₂):
-  lang_semantics ([loc x . C]) ty (s₁{x ↦ v}) (s₂{x ↦ v})
+-- | local_var {C s₁ s₂ ty} (x: string) (v: ℕ) (h: lang_semantics C ty s₁ s₂):
+--   lang_semantics ([loc x . C]) ty (s₁{x ↦ v}) (s₂{x ↦ v})
 
 /-! # Free-/
 
@@ -168,7 +168,7 @@ def stmt.Free: stmt → set string
 | (C₁ <+> C₂)               := (stmt.Free C₁) ∪ (stmt.Free C₂)
 | (C**)                     := stmt.Free C
 -- | [loc z . C]               := (stmt.Free C)
-| [loc z . C]               := (stmt.Free C) \ {z}
+-- | [loc z . C]               := (stmt.Free C) \ {z}
 | stmt.error                := {}
 | (stmt.assumes P)          := prop.Free P
 
@@ -195,7 +195,7 @@ def stmt.substitute : string → string → stmt → stmt
 | x y (C₁ ;; C₂)                := (stmt.substitute x y C₁) ;; (stmt.substitute x y C₂)
 | x y (C₁ <+> C₂)               := (stmt.substitute x y C₁) <+> (stmt.substitute x y C₂)
 | x y (C**)                     := (stmt.substitute x y C)**
-| x y [loc z . C]               := if x = z then [loc x . C] else [loc z . (stmt.substitute x y C)]
+-- | x y [loc z . C]               := if x = z then [loc x . C] else [loc z . (stmt.substitute x y C)]
 -- | x y [loc z . C]               := if x = z then [loc x . C] else (if y = z then C else [loc z . (stmt.substitute x y C)])
 | x y stmt.error                := stmt.error
 | x y (stmt.assumes P)          := stmt.assumes (P[y//x])
@@ -213,7 +213,7 @@ def Mod: stmt -> set string
 | (IncLoLang.stmt.non_det_assign x) := {x}
 | (IncLoLang.stmt.assumes _) := {}
 | (IncLoLang.stmt.error) := {}
-| (IncLoLang.stmt.local_var x C) := Mod C \ {x}
+-- | (IncLoLang.stmt.local_var x C) := Mod C \ {x}
 
 lemma mod_elem_left_elem_seq (C₁ C₂: stmt):
    Mod C₁ ⊆ Mod (C₁ ;; C₂):=
@@ -320,11 +320,11 @@ begin
     rw stmt.Free,
     exact h,
   },
-  case stmt.local_var {
-    rw Mod,
-    rw stmt.Free,
-    exact set.diff_subset_diff_left C_ih,
-  },
+  -- case stmt.local_var {
+  --   rw Mod,
+  --   rw stmt.Free,
+  --   exact set.diff_subset_diff_left C_ih,
+  -- },
   case stmt.error {
     rw Mod,
     rw stmt.Free,
@@ -508,42 +508,42 @@ begin
       { exact lang_semantics.seq_er_1 ( h₂_i_ih σ σ' LogicType.er h_H1 ), }
     }
   },
-  case stmt.local_var {
-    intros h₁ σ σ' ty v,
-    rw stmt.Free at h₁,
-    by_cases H: x = z,
-    {
-      cases H,
-      intro h,
-      cases h,
-      rw ← state.update,
-      rw ← state.update,
-      rw assign_order_eq,
-      rw assign_order_eq,
-      exact lang_semantics.local_var x v h_h,
-    },
-    {
-      have h₂: x ∉ C.Free, {
-        by_contra,
-        apply h₁,
-        split,
-        { exact h, },
-        { 
-          by_contra, 
-          apply H, 
-          exact set.mem_singleton_iff.1 h,
-        },
-      },
-      specialize C_ih h₂,
-      intro h,
-      cases h,
-      rw ← state.update,
-      rw ← state.update,
-      rw assign_order (ne.symm H),
-      rw assign_order (ne.symm H),
-      exact lang_semantics.local_var _ _ (C_ih h_s₁ h_s₂ ty v h_h)
-    },
-  },
+  -- case stmt.local_var {
+  --   intros h₁ σ σ' ty v,
+  --   rw stmt.Free at h₁,
+  --   by_cases H: x = z,
+  --   {
+  --     cases H,
+  --     intro h,
+  --     cases h,
+  --     rw ← state.update,
+  --     rw ← state.update,
+  --     rw assign_order_eq,
+  --     rw assign_order_eq,
+  --     exact lang_semantics.local_var x v h_h,
+  --   },
+  --   {
+  --     have h₂: x ∉ C.Free, {
+  --       by_contra,
+  --       apply h₁,
+  --       split,
+  --       { exact h, },
+  --       { 
+  --         by_contra, 
+  --         apply H, 
+  --         exact set.mem_singleton_iff.1 h,
+  --       },
+  --     },
+  --     specialize C_ih h₂,
+  --     intro h,
+  --     cases h,
+  --     rw ← state.update,
+  --     rw ← state.update,
+  --     rw assign_order (ne.symm H),
+  --     rw assign_order (ne.symm H),
+  --     exact lang_semantics.local_var _ _ (C_ih h_s₁ h_s₂ ty v h_h)
+  --   },
+  -- },
   case stmt.error {
     intros h₁ σ σ' ty v h,
     cases h,
@@ -633,7 +633,7 @@ begin
 end
 
 lemma assign_case {ty y x z e} {σ σ' : state} (Hyx: y ≠ x) (Hfreey: y ∉ ([z ↣ e].Free)):
-  lang_semantics ([z ↣ e]) ty (σ) (σ') ↔
+  lang_semantics ([z ↣ e]) ty (σ) (σ') →  
     lang_semantics ([z ↣ e]{y // x}) ty (σ⟨ y // x⟩) (σ'⟨ y // x ⟩) :=
 begin
   have H := (set.compl_subset_compl.mpr free_assign) Hfreey,
@@ -646,99 +646,73 @@ begin
     finish,
   },
 
-  split, {
-    sorry,
-    -- intro hls,
-    -- cases hls,
-    -- cases hls,
-    -- rw stmt.substitute,
+  intro hls,
+  cases hls,
+  cases hls,
+  rw stmt.substitute,
 
-    -- by_cases hx: x = z,
-    -- {
-    --   rw if_pos hx,
-    --   cases hx,
-    --   rw ← state.update,
-    --   rw expression.substitute,
-    --   simp,
+  by_cases hx: x = z,
+  {
+    rw if_pos hx,
+    cases hx,
+    rw ← state.update,
+    rw expression.substitute,
+    simp,
 
-    --   have H: σ{x ↦ e σ}⟨y//x⟩= σ⟨y//x⟩{y ↦ (λ (σ : state), e (σ⟨x//y⟩)) (σ⟨y//x⟩)}, 
-    --   {
-    --     ext z,
-    --     simp,
+    have H: σ{x ↦ e σ}⟨y//x⟩= σ⟨y//x⟩{y ↦ (λ (σ : state), e (σ⟨x//y⟩)) (σ⟨y//x⟩)}, 
+    {
+      ext z,
+      simp,
 
-    --     unfold state.update,
-    --     unfold state.substitute,
-    --     by_cases hx: x = z,
-    --     {finish,},
-    --     {
-    --       by_cases hy: y = z,
-    --       {
-    --         cases hy,
-    --         simp,
-    --         finish,
-    --       },
-    --       {
-    --         simp,
-    --         unfold state.update,
-    --         finish,
-    --       },
-    --     }
-    --   },
-      
-    --   rw H,
-    --   exact lang_semantics.assign,
-    -- },
-    -- {
-    --   rw if_neg hx,
-    --   rw ← state.update,
-    --   rw state.substitute,
-    --   simp,
-    --   rw assign_order (ne.symm H₂),
-    --   rw assign_order (ne.symm hx),
-    --   have H: σ{z ↦ e σ} x = σ x, {
-    --     funext, finish,
-    --   },
-    --   rw H,
-    --   rw expression.substitute,
-    --   have H: e σ = (λ (σ : state), e (σ⟨x//y⟩)) (σ{y ↦ σ x}{x ↦ 0}), {
-    --     simp,
-    --     rw state.substitute,
-    --     simp,
-    --     rw assign_order Hyx,
-    --     rw assign_order_eq,
-    --     have H: σ{x ↦ σ{y ↦ σ x}{x ↦ 0} y} = σ, {
-    --       funext, finish,
-    --     },
-    --     rw H,
-    --     exact H₁ σ 0,
-    --   },
-    --   rw H,
-    --   exact lang_semantics.assign,
-    -- },
+      unfold state.update,
+      unfold state.substitute,
+      by_cases hx: x = z,
+      {finish,},
+      {
+        by_cases hy: y = z,
+        {
+          cases hy,
+          simp,
+          finish,
+        },
+        {
+          simp,
+          unfold state.update,
+          finish,
+        },
+      }
+    },
+    
+    rw H,
+    exact lang_semantics.assign,
   },
   {
-    intros hls,
-    rw stmt.substitute at hls,
-
-    by_cases hx: x = z,
-    {
-      cases hx,
-      rw if_pos hx at hls,
-      have Hls2 := (assign_semantics hls).1,
-      have hty := (assign_semantics hls).2,
-      cases hty,
-
-      have H: σ' = σ{x ↦ e σ}, {
-        funext,
-        rw state.substitute at Hls2,
-        simp at Hls2,
-        by_cases x_1 = y,
-        
+    rw if_neg hx,
+    rw ← state.update,
+    rw state.substitute,
+    simp,
+    rw assign_order (ne.symm H₂),
+    rw assign_order (ne.symm hx),
+    have H: σ{z ↦ e σ} x = σ x, {
+      funext, finish,
+    },
+    rw H,
+    rw expression.substitute,
+    have H: e σ = (λ (σ : state), e (σ⟨x//y⟩)) (σ{y ↦ σ x}{x ↦ 0}), {
+      simp,
+      rw state.substitute,
+      simp,
+      rw assign_order Hyx,
+      rw assign_order_eq,
+      have H: σ{x ↦ σ{y ↦ σ x}{x ↦ 0} y} = σ, {
+        funext, finish,
       },
       rw H,
-      exact lang_semantics.assign,
+      exact H₁ σ 0,
     },
-  }
+    rw H,
+    exact lang_semantics.assign,
+  },
 end
 
 lemma substitution_rule {ty C y x} {σ σ' : state} (Hyx: y ≠ x) (Hfreey: y ∉ stmt.Free C):
@@ -752,8 +726,8 @@ begin
   induction C with z e z 
     C₁ C₂ hC₁ hC₂
     C₁ C₂ hC₁ hC₂
-    C hC
-    z C hC,
+    C hC,
+    -- z C hC,
   case stmt.skip {
     -- Skip case is trivial as σ = σ'
     intros _ σ _ h,
@@ -893,73 +867,73 @@ begin
       },
     },
   },
-  {
-    intros ty σ σ' hls,
-    cases hls,
-    rw stmt.substitute,
-    by_cases x = z,
-    {
-      cases h,
-      rw if_pos h,
-      rw stmt.Free at Hfreey,
-      have H : y ∉ C.Free, { finish, },
-      rw ← state.update,
-      rw ← state.update,
-      rw state.substitute,
-      simp,
-      have H₂ := free_language_semantics C y H,
-      rw ← assign_order Hyx,
-      rw ← assign_order Hyx,
-      rw assign_order_eq,
-      rw assign_order_eq,
-      specialize H₂ hls_s₁ hls_s₂ ty hls_v hls_h, 
-      exact lang_semantics.local_var _ _ H₂,
-    },
-    {
-      rw if_neg h,
-      rw stmt.Free at Hfreey,
-      by_cases y = z,
-      {
-        cases h,
-        rw ← state.update,
-        rw state.substitute,
-        rw ← state.update,
-        simp,
-        have H1: hls_s₁{y ↦ hls_v} x = hls_s₁ x, { unfold state.update, finish, },
-        have H2: hls_s₂{y ↦ hls_v} x = hls_s₂ x, { unfold state.update, finish, },
-        rw H1, rw H2,
-        sorry,
-         -- [loc z. z = 5]
-         -- [loc z. x = 5](z//x)
-         -- [loc z. z = 5](z//x) !! Need to move to fresh
-        -- exact lang_semantic.local_var y hls_v (hC Hfreey hls_h),
-        -- rw stmt.substitute,
-        -- x ≠ b (σ1, σ2) ∈ ⟦local x . C⟧ and y ∉ Free C ⇒ (σ1(y/b), σ2(y/b)) ∈ ⟦local x . C(y/b)⟧
-        -- ({b = 1}, {b = 2}) ∈ ⟦local y . b = 2⟧ ⇒ ({y = 1}, {y = 2}) ∈ ⟦local y . y = 2⟧
-      },
-      {
-        have H: y ∉ C.Free, { by_contra, finish, },
-        specialize hC H hls_h,
-        rw ← state.update,
-        rw ← state.update,
-        simp,
-        have H1: ∀ σ, ((σ{z ↦ hls_v})⟨y//x⟩) = ((σ⟨y//x⟩){z ↦ hls_v}), {
-          intro σ,
-          rw state.substitute,
-          funext,
-          simp,
-          unfold state.update,
-          by_cases name' = x, { cases h, finish, },
-          by_cases name' = y, { cases h, finish, },
-          by_cases name' = z, { cases h, finish, },
-          finish,
-        },
-        rw (H1 hls_s₁),
-        rw (H1 hls_s₂),
-        exact lang_semantics.local_var _ _ hC,
-      },
-    },
-  },
+  -- case stmt.local_var {
+  --   intros ty σ σ' hls,
+  --   cases hls,
+  --   rw stmt.substitute,
+  --   by_cases x = z,
+  --   {
+  --     cases h,
+  --     rw if_pos h,
+  --     rw stmt.Free at Hfreey,
+  --     have H : y ∉ C.Free, { finish, },
+  --     rw ← state.update,
+  --     rw ← state.update,
+  --     rw state.substitute,
+  --     simp,
+  --     have H₂ := free_language_semantics C y H,
+  --     rw ← assign_order Hyx,
+  --     rw ← assign_order Hyx,
+  --     rw assign_order_eq,
+  --     rw assign_order_eq,
+  --     specialize H₂ hls_s₁ hls_s₂ ty hls_v hls_h, 
+  --     exact lang_semantics.local_var _ _ H₂,
+  --   },
+  --   {
+  --     rw if_neg h,
+  --     rw stmt.Free at Hfreey,
+  --     by_cases y = z,
+  --     {
+  --       cases h,
+  --       rw ← state.update,
+  --       rw state.substitute,
+  --       rw ← state.update,
+  --       simp,
+  --       have H1: hls_s₁{y ↦ hls_v} x = hls_s₁ x, { unfold state.update, finish, },
+  --       have H2: hls_s₂{y ↦ hls_v} x = hls_s₂ x, { unfold state.update, finish, },
+  --       rw H1, rw H2,
+  --       sorry,
+  --        -- [loc z. z = 5]
+  --        -- [loc z. x = 5](z//x)
+  --        -- [loc z. z = 5](z//x) !! Need to move to fresh
+  --       -- exact lang_semantic.local_var y hls_v (hC Hfreey hls_h),
+  --       -- rw stmt.substitute,
+  --       -- x ≠ b (σ1, σ2) ∈ ⟦local x . C⟧ and y ∉ Free C ⇒ (σ1(y/b), σ2(y/b)) ∈ ⟦local x . C(y/b)⟧
+  --       -- ({b = 1}, {b = 2}) ∈ ⟦local y . b = 2⟧ ⇒ ({y = 1}, {y = 2}) ∈ ⟦local y . y = 2⟧
+  --     },
+  --     {
+  --       have H: y ∉ C.Free, { by_contra, finish, },
+  --       specialize hC H hls_h,
+  --       rw ← state.update,
+  --       rw ← state.update,
+  --       simp,
+  --       have H1: ∀ σ, ((σ{z ↦ hls_v})⟨y//x⟩) = ((σ⟨y//x⟩){z ↦ hls_v}), {
+  --         intro σ,
+  --         rw state.substitute,
+  --         funext,
+  --         simp,
+  --         unfold state.update,
+  --         by_cases name' = x, { cases h, finish, },
+  --         by_cases name' = y, { cases h, finish, },
+  --         by_cases name' = z, { cases h, finish, },
+  --         finish,
+  --       },
+  --       rw (H1 hls_s₁),
+  --       rw (H1 hls_s₂),
+  --       exact lang_semantics.local_var _ _ hC,
+  --     },
+  --   },
+  -- },
   {
     intros ty σ σ' hls,
     cases hls,
@@ -988,257 +962,111 @@ begin
   },
 end
 
-lemma substitution_rule_2 {ty C y x} {σ σ' : state} (Hyx: y ≠ x) (Hfreey: y ∉ stmt.Free C):
-  lang_semantics (C{y // x}) ty (σ) (σ') →
-    -- If C can take σ to σ'
-    lang_semantics C ty (σ{x ↦ σ' y}) (σ'{x ↦ σ' y}) :=
-    -- Then C(y/x) can take σ with y set to x's value in σ to σ' with y set to x's value in σ' 
-begin
-  revert ty σ σ',
-
-  induction C with z e z 
+lemma stmt_free_unchanged {x: string} {C: stmt} {σ σ': state} {ty: LogicType}: 
+  (lang_semantics C ty σ σ') ∧ (x ∉ C.Free) → σ x = σ' x :=
+begin 
+  revert σ σ' ty,
+  induction C with 
+    y e
+    y
     C₁ C₂ hC₁ hC₂
     C₁ C₂ hC₁ hC₂
-    C hC
-    z C hC,
+    C Ch,
   case stmt.skip {
-    -- Skip case is trivial as σ = σ'
-    intros _ σ _ h,
-    cases h,
-    exact lang_semantics.skip,
+    rintros σ σ' ty ⟨ hls, hxFree ⟩,
+    cases hls,
+    refl,
   },
   case stmt.assign {
-    intros ty σ σ' hls,
-    exact assign_case Hyx Hfreey hls,
+    rintros σ σ' ty ⟨ hls, hxFree ⟩,
+    cases hls,
+    unfold stmt.Free at hxFree,
+    have H: x ≠ y, { finish, },
+    simp,
+    rw if_neg H,
   },
   case stmt.non_det_assign {
-    intros ty σ σ' hls,
-
-    by_cases x = z,
-    {
-      cases h,
-      rw stmt.substitute,
-      cases hls,
-      unfold state.substitute,
-      rw if_pos (rfl),
-      rw ← state.update,
-      rw ← assign_order Hyx,
-      rw if_pos (rfl),
-      simp,
-      rw assign_order Hyx,
-      rw assign_order Hyx,
-      have H: σ{x ↦ 0}{y ↦ hls_v} = σ{x ↦ 0}{y ↦ σ x}{y ↦ hls_v}, { rw assign_order_eq, },
-      rw H,
-      exact lang_semantics.non_det_assign hls_v,
-    },
-    {
-      rw stmt.substitute,
-      cases hls,
-      unfold state.substitute,
-      rw if_neg h,
-      rw ← state.update,
-      rw if_neg h,
-      by_cases H₂: z = y,
-      {
-        cases H₂,
-        rw assign_order_eq,
-        rw assign_order (ne.symm h),
-        have H: σ{x ↦ 0}{y ↦ σ x} = σ{x ↦ 0}{y ↦ σ x}{y ↦ σ x}, { rw assign_order_eq, },
-        nth_rewrite 1 H,
-        exact lang_semantics.non_det_assign (σ x),
-      },
-      {
-        rw assign_order H₂,
-        rw assign_order (ne.symm h),
-        exact lang_semantics.non_det_assign hls_v,
-      }
-    },
+    rintros σ σ' ty ⟨ hls, hxFree ⟩,
+    cases hls,
+    unfold stmt.Free at hxFree,
+    have H: x ≠ y, { finish, },
+    simp,
+    rw if_neg H,
   },
   case stmt.seq {
-    intros ty σ σ' hls,
+    rintros σ σ' ty ⟨ hls, hxFree ⟩,
+    have H₁: x ∉ C₁.Free, {by_contra, apply hxFree, left, exact h,},
+    have H₂: x ∉ C₂.Free, {by_contra, apply hxFree, right, exact h,},
     cases hls,
     {
-      specialize hC₁ (by {
-        by_contra,
-        apply Hfreey,
-        left,
-        exact h,
-      }) hls_H1,
-      specialize hC₂ (by {
-        by_contra,
-        apply Hfreey,
-        right,
-        exact h,
-      }) hls_H2,
-      rw stmt.substitute,
-      exact lang_semantics.seq_ty hC₁ hC₂,
+      specialize hC₁ (⟨hls_H1, H₁⟩),
+      specialize hC₂ (⟨hls_H2, H₂⟩),
+      rw hC₁,
+      exact hC₂,
     },
     {
-      specialize hC₁ (by {
-        by_contra,
-        apply Hfreey,
-        left,
-        exact h,
-      }) hls_H1,
-      rw stmt.substitute,
-      exact lang_semantics.seq_er_1 hC₁,
-    }
+      exact hC₁ (⟨hls_H1, H₁⟩),
+    },
   },
   case stmt.choice {
-    intros ty σ σ' hls,
+    rintros σ σ' ty ⟨ hls, hxFree ⟩,
+    have H₁: x ∉ C₁.Free, {by_contra, apply hxFree, left, exact h,},
+    have H₂: x ∉ C₂.Free, {by_contra, apply hxFree, right, exact h,},
     cases hls,
     {
-      specialize hC₁ (by {
-        by_contra,
-        apply Hfreey,
-        left,
-        exact h,
-      }) hls_h,
-      rw stmt.substitute,
-      exact lang_semantics.choice_left hC₁,
+      specialize hC₁ (⟨hls_h, H₁⟩),
+      exact hC₁,
     },
     {
-      specialize hC₂ (by {
-        by_contra,
-        apply Hfreey,
-        right,
-        exact h,
-      }) hls_h,
-      rw stmt.substitute,
-      exact lang_semantics.choice_right hC₂,
-    }
+      specialize hC₂ (⟨hls_h, H₂⟩),
+      exact hC₂,
+    },
   },
   case stmt.star {
-    intros ty σ σ' hls,
+    rintros σ σ' ty ⟨ hls, hxFree ⟩,
     cases hls,
-    rw stmt.substitute,
-    use hls_i,
-    revert ty σ σ' ,
-    induction hls_i,
+    revert ty σ σ', 
+    induction hls_i with n hC' hC',
     {
-      intros ty σ σ' hls_h,
+      intros _ _ _ hls_h,
       rw repeat at hls_h,
       cases hls_h,
-      rw repeat,
-      exact lang_semantics.skip,
+      refl,
     },
     {
-      intros ty σ σ' hls_h,
-      rw repeat at hls_h,
-      cases hls_h,
+      intros ty σ σ' hls,
+      rw repeat at hls,
+      rw stmt.Free at hxFree,
+      cases hls,
       {
-        specialize hls_i_ih hls_h_H1,
-        rw stmt.Free at Hfreey,
-        specialize hC Hfreey hls_h_H2, 
-        rw repeat,
-        exact lang_semantics.seq_ty hls_i_ih hC,
+        specialize Ch (⟨hls_H2, hxFree⟩),
+        specialize hC' hls_H1,
+        rw hC',
+        exact Ch,
       },
       {
-        specialize hls_i_ih hls_h_H1,
-        rw repeat,
-        exact lang_semantics.seq_er_1 hls_i_ih,
+        specialize hC' hls_H1,
+        exact hC',
       },
-    },
+    }
   },
-  {
-    intros ty σ σ' hls,
+  case stmt.error {
+    rintros σ σ' ty ⟨ hls, hxFree ⟩,
     cases hls,
-    rw stmt.substitute,
-    by_cases x = z,
-    {
-      cases h,
-      rw if_pos h,
-      rw stmt.Free at Hfreey,
-      have H : y ∉ C.Free, { finish, },
-      rw ← state.update,
-      rw ← state.update,
-      rw state.substitute,
-      simp,
-      have H₂ := free_language_semantics C y H,
-      rw ← assign_order Hyx,
-      rw ← assign_order Hyx,
-      rw assign_order_eq,
-      rw assign_order_eq,
-      specialize H₂ hls_s₁ hls_s₂ ty hls_v hls_h, 
-      exact lang_semantics.local_var _ _ H₂,
-    },
-    {
-      rw if_neg h,
-      rw stmt.Free at Hfreey,
-      by_cases y = z,
-      {
-        cases h,
-        rw ← state.update,
-        rw state.substitute,
-        rw ← state.update,
-        simp,
-        have H1: hls_s₁{y ↦ hls_v} x = hls_s₁ x, { unfold state.update, finish, },
-        have H2: hls_s₂{y ↦ hls_v} x = hls_s₂ x, { unfold state.update, finish, },
-        rw H1, rw H2,
-        sorry,
-         -- [loc z. z = 5]
-         -- [loc z. x = 5](z//x)
-         -- [loc z. z = 5](z//x) !! Need to move to fresh
-        -- exact lang_semantic.local_var y hls_v (hC Hfreey hls_h),
-        -- rw stmt.substitute,
-        -- x ≠ b (σ1, σ2) ∈ ⟦local x . C⟧ and y ∉ Free C ⇒ (σ1(y/b), σ2(y/b)) ∈ ⟦local x . C(y/b)⟧
-        -- ({b = 1}, {b = 2}) ∈ ⟦local y . b = 2⟧ ⇒ ({y = 1}, {y = 2}) ∈ ⟦local y . y = 2⟧
-      },
-      {
-        have H: y ∉ C.Free, { by_contra, finish, },
-        specialize hC H hls_h,
-        rw ← state.update,
-        rw ← state.update,
-        simp,
-        have H1: ∀ σ, ((σ{z ↦ hls_v})⟨y//x⟩) = ((σ⟨y//x⟩){z ↦ hls_v}), {
-          intro σ,
-          rw state.substitute,
-          funext,
-          simp,
-          unfold state.update,
-          by_cases name' = x, { cases h, finish, },
-          by_cases name' = y, { cases h, finish, },
-          by_cases name' = z, { cases h, finish, },
-          finish,
-        },
-        rw (H1 hls_s₁),
-        rw (H1 hls_s₂),
-        exact lang_semantics.local_var _ _ hC,
-      },
-    },
+    refl,
   },
-  {
-    intros ty σ σ' hls,
+  case stmt.assumes {
+    rintros σ σ' ty ⟨ hls, hxFree ⟩,
     cases hls,
-    rw stmt.substitute,
-    exact lang_semantics.error,  
-  },
-  {
-    intros ty σ σ' hls,
-    cases hls,
-    rw stmt.substitute,
-    have H: (C[y//x]) (σ⟨y//x⟩), { 
-      unfold prop.substitute,
-      unfold state.substitute,
-      rw assign_order_eq,
-      have H: σ{y ↦ σ x}{x ↦ σ{y ↦ σ x}{x ↦ 0} y} = σ{y ↦ σ x}, {
-        unfold state.update,
-        funext,
-        finish,
-      },
-      rw H,
-      rw stmt.Free at Hfreey,
-      apply (not_free_prop Hfreey σ (σ x)).1,
-      exact hls_h,
-    },
-    exact lang_semantics.assumes_ok H,
+    refl,
   },
 end
 
-lemma substitution_free {x y : string} {C: stmt}:
-  (x ∈ C.Free) → (y ∉ C.Free) → (y ∈ ((C{y // x}).Free)) :=
-begin
+lemma for_all_free_expression {e: expression} {σ σ': state } (H: ∀ x ∈ e.Free, σ x = σ' x): e σ = e σ' :=
+begin 
+  -- Help??
   sorry,
+  -- trivial,
 end
 
 end IncLoLang
